---
aliases: []
tags:
  - date/2023/10/18
  - languages/in/English
  - questions/mathematics/combinatorics
---

Prove $$\forall{}n\in\mathbb{Z}^+\sum_{k=0}^n(-1)^k\binom{n}k=0$$.

> [!success]- solution
>
> $$\begin{aligned}
0&=(1+(-1))^n\\
&=\sum_{k=0}^n\binom{n}k(-1)^k(1)^{n-k}\\
&=\sum_{k=0}^n(-1)^k\binom{n}k
\end{aligned}$$

> [!success]- solution 2
>
> $$\begin{aligned}
&\text{For odd }n\text{, let }n=2m+1\text{.}\\
&\begin{aligned}\sum_{k=0}^n(-1)^k\binom{n}k&=\sum_{k=0}^{2m+1}(-1)^k\binom{2m+1}k\\
&=\sum_{k=0}^m(-1)^k\binom{2m+1}k+\sum_{k=m+1}^{2m+1}(-1)^k\binom{2m+1}k\\
&=\sum_{k=0}^m(-1)^k\binom{2m+1}k+\sum_{k=m+1}^{2m+1}(-1)^k\binom{2m+1}{2m+1-k}\\
&=\sum_{k=0}^m(-1)^k\binom{2m+1}k+\sum_{k=0}^{m}(-1)^{m+1+k}\binom{2m+1}{2m+1-(m+1+k)}\\
&=\sum_{k=0}^m(-1)^k\binom{2m+1}k-\sum_{k=0}^{m}(-1)^{m+k}\binom{2m+1}{m-k}\\
&=\sum_{k=0}^m(-1)^k\binom{2m+1}k-\sum_{k=0}^{m}(-1)^{m+(m-k)}\binom{2m+1}{m-(m-k)}\\
&=\sum_{k=0}^m(-1)^k\binom{2m+1}k-\sum_{k=0}^{m}(-1)^{2m-k}\binom{2m+1}k\\
&=\sum_{k=0}^m(-1)^k\binom{2m+1}k-\sum_{k=0}^{m}(-1)^k\binom{2m+1}k\\
&=0\end{aligned}\\
&\text{For even }n\text{, let }n=2m\text{.}\\
&\begin{aligned}\sum_{k=0}^n(-1)^k\binom{n}k&=\sum_{k=0}^{2m}(-1)^k\binom{2m}k\\
&=\sum_{k=0}^{2m}(-1)^k\left(\binom{2m+1}k-\binom{2m}{k-1}\right)\\
&=\sum_{k=0}^{2m}(-1)^k\binom{2m+1}k-\sum_{k=0}^{2m}(-1)^k\binom{2m}{k-1}\\
&=\sum_{k=0}^{2m+1}(-1)^k\binom{2m+1}k-(-1)^{2m+1}\binom{2m+1}{2m+1}-\sum_{k=1}^{2m}(-1)^k\binom{2m}{k-1}-(-1)^k\binom{2m}{-1}\\
&=0+1-\sum_{k=1}^{2m}(-1)^k\binom{2m}{k-1}-0\\
&=1+\sum_{k=0}^{2m-1}(-1)^k\binom{2m}{k}\\
&=1+\sum_{k=0}^{2m-1}(-1)^k\binom{2m-1}{k}+\sum_{k=0}^{2m-1}(-1)^k\binom{2m-1}{k-1}\\
&=1+0+\sum_{k=1}^{2m}(-1)^k\binom{2m-1}{k-1}+(-1)^0\binom{2m-1}{-1}-(-1)^{2m}\binom{2m-1}{2m-1}\\
&=1-\sum_{k=0}^{2m-1}(-1)^k\binom{2m-1}{k}+0-1\\
&=1-0-1\\
&=0\end{aligned}
\end{aligned}$$
