---
aliases: []
tags:
  - date/2023/09/24
  - flashcard/special/questions/2023-09-24T111551_871_0800
  - language/in/English
  - question/mathematics/trigonometry
---

# 2023-09-24T111551.871+0800

Express $\tan3x$ in terms of $\tan{x}$. Hence, prove $\tan^2\frac\pi5=5-2\sqrt5$ and $\tan^2\frac{2\pi}5=5+2\sqrt5$.

## strategy

- inspecting "Express $\tan3x$ in terms of $\tan{x}$." :: Apply the angle sum formula ($\tan(a \pm b) = \frac {\tan a \pm \tan b} {1 \mp \tan a \tan b}$) twice. <!--SR:!2024-07-06,4,270-->
- inspecting "Hence, prove $\tan^2\frac\pi5=5-2\sqrt5$ and $\tan^2\frac{2\pi}5=5+2\sqrt5$." after expressing $\tan 3x$ in terms of $\tan x$ :: Realize that $\tan^2 \frac {2\pi} 5 = \tan^2 \frac {3\pi} 5$. Let $x = \frac \pi 5$ to setup an equation using the expression for $\tan 3x$ to find $\tan^2 \frac \pi 5$. Then find $\tan^2 \frac {2\pi} 5$. <!--SR:!2024-07-05,3,250-->

## solution

$$\begin{aligned}
\tan2x&=\frac{2\tan{x} }{1-\tan^2x}\\
\tan3x&=\frac{\tan{x}+\tan2x}{1-\tan{x}\tan2x}\\
&=\frac{\tan{x}+\frac{2\tan{x} }{1-\tan^2x} }{1-\tan{x}\left(\frac{2\tan{x} }{1-\tan^2x}\right)}\\
&=\frac{\frac{3\tan{x}-\tan^3x}{1-\tan^2x} }{\frac{1-3\tan^2x}{1-\tan^2x} }\\
&=\frac{3\tan{x}-\tan^3x}{1-3\tan^2x}\\
\alpha&\overset{\text{def} }=\frac\pi5\\
\tan\frac{2\pi}5&=-\tan\frac{3\pi}5\\
\tan2\alpha&=-\tan3\alpha\\
\frac{2\tan\alpha}{1-\tan^2\alpha}&=\frac{\tan^3\alpha-3\tan\alpha}{1-3\tan^2\alpha}\\
2\tan\alpha-6\tan^3\alpha&=\tan^3\alpha-3\tan\alpha-\tan^5\alpha+3\tan^3\alpha\\
\tan^5\alpha-10\tan^3\alpha+5\tan\alpha&=0\\
\tan\alpha\left(\tan^2\alpha-5+2\sqrt5\right)\left(\tan^2\alpha-5-2\sqrt5\right)&=0\\
\left(\tan^2\alpha-5+2\sqrt5\right)\left(\tan^2\alpha-5-2\sqrt5\right)&=0 && \left(\tan\alpha\ne0\right)\\
\tan^2\alpha&=5\pm2\sqrt5\\
\tan^2\alpha&=5-2\sqrt5 && (\left|\tan\alpha\right|<1,\tan^2\alpha<1)\\
\tan^22\alpha&=\left(\frac{2\tan\alpha}{1-\tan^2\alpha}\right)^2\\
&=\frac{4\tan^2\alpha}{1-2\tan^2\alpha+\tan^4\alpha}\\
&=\frac{20-8\sqrt5}{1-10+4\sqrt5+25-20\sqrt5+20}\\
&=\frac{20-8\sqrt5}{36-16\sqrt5}\\
&=\frac{5-2\sqrt5}{9-4\sqrt5}\\
&=\frac{\left(5-2\sqrt5\right)\left(9+4\sqrt5\right)}{81-80}\\
&=45+2\sqrt5-40\\
&=5+2\sqrt5\\
\left(\tan^2\frac\pi5,\tan^2\frac{2\pi}5\right)&=\left(5-2\sqrt5,5+2\sqrt5\right)\\
\end{aligned}$$
