---
aliases: []
tags:
  - date/2023/11/22
  - language/in/English
  - question/mathematics/complex_analysis
---

Prove that $$\frac{a+bi}{c+di}=\frac{ac+bd}{c^2+d^2}+i\frac{bc-ad}{c^2+d^2},\text{where }a,b,c,d\in\mathbb{R}$$.

> [!success]- solution
>
> $$\begin{aligned}
\frac{a+bi}{c+di}&=\frac{(a+bi)(c-di)}{(c+di)(c-di)}\\
&=\frac{ac-adi+bci+bd}{c^2+d^2}\\
&=\frac{(ac+bd)+(bc-ad)i}{c^2+d^2}\\
&=\frac{ac+bd}{c^2+d^2}+i\frac{bc-ad}{c^2+d^2}
\end{aligned}$$

<!-- markdownlint MD028 -->

> [!success]- solution 2
>
> $$\begin{aligned}
\frac{a+bi}{c+di}&=\frac{\sqrt{a^2+b^2}(\cos(\operatorname{atan2}(b,a))+i\sin(\operatorname{atan2}(b,a)))}{\sqrt{c^2+d^2}(\cos(\operatorname{atan2}(d,c))+i\sin(\operatorname{atan2}(d,c)))}\\
&=\frac{\sqrt{a^2+b^2}e^{i\operatorname{atan2}(b,a)}}{\sqrt{c^2+d^2}e^{i\operatorname{atan2}(d,c)}}\\
&=\frac{\sqrt{a^2+b^2}}{\sqrt{c^2+d^2}}e^{i(\operatorname{atan2}(b,a)-\operatorname{atan2}(d,c))}\\
&=\frac{\sqrt{a^2+b^2}}{\sqrt{c^2+d^2}}e^{i\operatorname{atan2}(bc-ad,ac+bd)}\\
&=\frac{\sqrt{a^2+b^2}}{\sqrt{c^2+d^2}}(\cos(\operatorname{atan2}(bc-ad,ac+bd))+i\sin(\operatorname{atan2}(bc-ad,ac+bd)))\\
&=\frac{\sqrt{a^2+b^2}}{\sqrt{c^2+d^2}}\left(\frac{ac+bd}{\sqrt{(bc-ad)^2+(ac+bd)^2}}+i\frac{bc-ad}{\sqrt{(bc-ad)^2+(ac+bd)^2}}\right)\\
&=\frac{\sqrt{\left(a^2+b^2\right)\left(c^2+d^2\right)}}{c^2+d^2}\left(\frac{ac+bd}{\sqrt{(bc-ad)^2+(ac+bd)^2}}+i\frac{bc-ad}{\sqrt{(bc-ad)^2+(ac+bd)^2}}\right)\\
&=\frac{\sqrt{a^2c^2+a^2d^2+b^2c^2+b^2d^2}}{c^2+d^2}\left(\frac{ac+bd}{\sqrt{b^2c^2+a^2d^2+a^2c^2+b^2d^2}}+i\frac{bc-ad}{\sqrt{b^2c^2+a^2d^2+a^2c^2+b^2d^2}}\right)\\
&=\frac{ac+bd}{c^2+d^2}+i\frac{bc-ad}{c^2+d^2}
\end{aligned}$$
