---
aliases: []
tags:
  - date/2023/12/07
  - flashcard/active/special/questions/2023-12-07T084120_499_0800
  - language/in/English
  - question/mathematics/calculus/differential
---

# 2023-12-07T084120.499+0800

Given a [twice-differentiable](../../general/differentiable%20function.md) $f$, prove that if $f(-x)=-f(x)$, then $f''(-x)=-f''(x)$.

## strategy

- inspecting "Given a [twice-differentiable](../../general/differentiable%20function.md) $f$, prove that if $f(-x)=-f(x)$, then $f''(-x)=-f''(x)$." :: Use the derivative definition twice.

## solution

$$\begin{aligned}
f'(x)&=\lim_{h\to0}\frac{f(x+h)-f(x)}h\\
f'(-x)&=\lim_{h\to0}\frac{f(-x+h)-f(-x)}h\\
&=\lim_{h\to0}\frac{-f(x-h)+f(x)}h\\
&=\lim_{h\to0}\frac{-f(x+h)+f(x)}{-h}\\
&=\lim_{h\to0}\frac{f(x+h)-f(x)}h\\
&=f'(x)\\
f''(x)&=\lim_{h\to0}\frac{f'(x+h)-f'(x)}h\\
f''(-x)&=\lim_{h\to0}\frac{f'(-x+h)-f'(-x)}h\\
&=\lim_{h\to0}\frac{f'(x-h)-f'(x)}h\\
&=\lim_{h\to0}\frac{f'(x+h)-f'(x)}{-h}\\
&=-f''(x)
\end{aligned}$$
