---
aliases: []
tags:
  - date/2023/11/21
  - language/in/English
  - question/mathematics/calculus/differential
  - question/mathematics/integral_transform
---

Solve $$f''(x)+2f'(x)+f(x)=0,x\in\mathbb{R}^+_0$$ using its [characteristic equation](../../general/characteristic%20equation%20(calculus).md). Then solve it again using the [Laplace transform](../../general/Laplace%20transform.md). Observe any relations between the results.

## solution

$$\begin{aligned}
&\text{Using the characteristic equation,}\\
&\begin{aligned}f''(x)+2f'(x)+f(x)&=0\\
r^2+2r+1&=0\\
(r+1)^2&=0\\
r&=-1\text{ (repeated)}\\
f(x)&=c_1e^{-x}+c_2xe^{-x}\end{aligned}\\
&\text{Using the Laplace transform,}\\
&\begin{aligned}f''(x)+2f'(x)+f(x)&=0\\
\begin{aligned}s^2\mathcal{L}\{f(x)\}-sf(0^-)-f'(0^-)\\+2s\mathcal{L}\{f(x)\}-2f(0^-)\\
+\mathcal{L}\{f(x)\}\end{aligned}&=\mathcal{L}\{0\}\\
\begin{aligned}\left(s^2+2s+1\right)\mathcal{L}\{f(x)\}\\-(s+2)f(0^-)\\-f'(0^-)\end{aligned}&=0\\
\mathcal{L}\{f(x)\}&=\frac{(s+2)f(0^-)+f'(0^-)}{s^2+2s+1}\\
&=\frac{(s+2)f(0^-)+f'(0^-)}{(s+1)^2}\\
&=\frac{s+1}{(s+1)^2}f(0^-)+\frac{1}{(s+1)^2}(f(0^-)+f'(0^-))\\
f(x)&=e^{-x}\cos(0x)\cdot{}u(x)\cdot{}f(0^-)+x^1e^{-x}\cdot{}u(x)\cdot(f(0^-)+f'(0^-))\\
&=f(0^-)e^{-x}+(f(0^-)+f'(0^-))xe^{-x} && (x\ge0\implies{}u(x)=1)\end{aligned}\\
&\text{It can be inferred that }c_1=f(0^-),c_2=f(0^-)+f'(0^-)\text{.}
\end{aligned}$$
