---
aliases: []
tags:
  - date/2024/02/17
  - flashcard/active/special/questions/2024-02-17T130838_403_0800
  - language/in/English
  - question/mathematics/matrix
---

# 2024-02-17T130838.403+0800

Let $A = \begin{bmatrix} 8 & 3 \\ -18 & -7 \end{bmatrix}, P = \begin{bmatrix} 1 & -1 \\ -2 & 3 \end{bmatrix}$. Given that $P^{-1} = \begin{bmatrix} 3 & 1 \\ 2 & 1 \end{bmatrix}, P^{-1}AP = \begin{bmatrix} 2 & 0 \\ 0 & -1 \end{bmatrix}$, find $$I_2 + A^2 + A^4 + \cdots + A^{2n}$$, where $n$ is a positive integer.

## tips

The [geometric sum](../../general/geometric%20series.md#sum) cannot be used as the matrix $A^2 - I_2$ is not invertible.

## strategy

- inspecting "$$I_2 + A^2 + A^4 + \cdots + A^{2n}$$" :@: Find the general expression for $A^{2i}$ for all integers $i \ge 0$. <!--SR:!2029-06-11,1399,350-->

## solution

$$\begin{aligned}
A^n & = PP^{-1}\left(APP^{-1}\right)^n \\
& = P\left(P^{-1}AP\right)^nP^{-1} \\
& = P \begin{bmatrix} 2 & 0 \\ 0 & -1 \end{bmatrix}^n P^{-1} \\
& = P \begin{bmatrix} 2^n & 0 \\ 0 & (-1)^n \end{bmatrix} P^{-1} \\
& = \begin{bmatrix} 1 & -1 \\ -2 & 3 \end{bmatrix} \begin{bmatrix} 2^n & 0 \\ 0 & (-1)^n \end{bmatrix} \begin{bmatrix} 3 & 1 \\ 2 & 1 \end{bmatrix} \\
& = \begin{bmatrix} 2^n & (-1)^{n + 1} \\ -2^{n + 1} & (-1)^n \cdot 3 \end{bmatrix} \begin{bmatrix} 3 & 1 \\ 2 & 1 \end{bmatrix} \\
& = \begin{bmatrix} 2^n \cdot 3 + (-1)^{n + 1} \cdot 2 & 2^n + (-1)^{n + 1} \\ -2^{n + 1} \cdot 3 + (-1)^n \cdot 6 & -2^{n + 1} + (-1)^n \cdot 3 \end{bmatrix} \\
& = \begin{bmatrix} 2^n \cdot 3 - (-1)^n \cdot 2 & 2^n - (-1)^n \\ -2^n \cdot 6 + (-1)^n \cdot 6 & -2^n \cdot 2 + (-1)^n \cdot 3 \end{bmatrix} \\
A^{2n} & = \begin{bmatrix} 2^{2n} \cdot 3 - 2 & 2^{2n} - 1 \\ -2^{2n} \cdot 6 + 6 & -2^{2n} \cdot 2 +  3 \end{bmatrix} \\
& = I_2 + \begin{bmatrix} 2^{2n} \cdot 3 - 3 & 2^{2n} - 1 \\ -2^{2n} \cdot 6 + 6 & -2^{2n} \cdot 2 +  2 \end{bmatrix} \\
& = I_2 + \left(2^{2n} - 1\right) \begin{bmatrix} 3 & 1 \\ -6 & -2 \end{bmatrix} \\
I_2 + A^2 + A^4 + \ldots + A^{2n} & = (n + 1) I_2 + \left(\frac {2^{2n + 2} - 1} {2^{2n} - 1} - (n + 1) \right) \begin{bmatrix} 3 & 1 \\ -6 & -2 \end{bmatrix} \\
& = (n + 1) \begin{bmatrix} -2 & -1 \\ 6 & 3 \end{bmatrix} + \frac {2^{2n + 2} - 1} {2^{2n} - 1} \begin{bmatrix} 3 & 1 \\ -6 & -2 \end{bmatrix}
\end{aligned}$$
