---
aliases: []
tags:
  - date/2024/02/07
  - flashcard/active/special/questions/2024-02-07T183935_701_0800
  - language/in/English
  - question/mathematics/calculus
---

# 2024-02-07T183935.701+0800

Given that $$\int _1 ^n \! \ln x \,\mathrm{d}x \le \sum _{k = 2} ^n \ln k \le \int _1 ^n \! \ln x \,\mathrm{d}x + \ln n \qquad n \in \mathbb{Z}_{\ge 2} \,,$$ show that $$\lim_{n \to \infty} \frac { \sqrt[n]{n!} } n = \frac 1 e \,.$$

## strategy

- inspecting "Given that $$\int _1 ^n \! \ln x \,\mathrm{d}x \le \sum _{k = 2} ^n \ln k \le \int _1 ^n \! \ln x \,\mathrm{d}x + \ln n \qquad n \in \mathbb{Z}_{\ge 2} \,,$$ show that $$\lim_{n \to \infty} \frac { \sqrt[n]{n!} } n = \frac 1 e \,.$$" :@: Taking the logarithm of the limit would probably yield something amenable to the above inequality... Further, such an inequality suggests squeeze theorem.

## solution

1. <span></span> $$\begin{aligned}
\int _1 ^n \! \ln x \,\mathrm{d}x & = [x \ln x] _1 ^n - \int_1 ^n \! x \,\mathrm{d}\ln x \\
& = n \ln n - \int _1 ^n \,\mathrm{d}x \\
& = n \ln n - n + 1 \\
\\
\lim_{n \to \infty} \frac { \sqrt[n]{n!} } n & = \exp \ln \lim_{n \to \infty} \frac { \sqrt[n]{n!} } n \\
& = \exp \lim_{n \to \infty} \ln \frac { \sqrt[n]{n!} } n && (\ln \text{ is continuous}) \\
& = \exp \lim_{n \to \infty} \left(\frac 1 n \sum _{k = 1} ^n \ln k - \ln n \right) \\
\exp \lim_{n \to \infty} \left(\frac 1 n \int _1 ^n \! \ln x \,\mathrm{d}x - \ln n \right)  & \le \exp \lim_{n \to \infty} \left(\frac 1 n \sum _{k = 2} ^n \ln k - \ln n \right) \le \exp \lim_{n \to \infty} \left(\frac 1 n \int _1 ^n \! \ln x \,\mathrm{d}x - \frac {n - 1} n \ln n \right) && \left( e^* \text{ is increasing} \right) \\
\exp \lim_{n \to \infty} \left(\ln n - 1 + \frac 1 n - \ln n \right)  & \le \exp \lim_{n \to \infty} \left(\frac 1 n \sum _{k = 2} ^n \ln k - \ln n \right) \le \exp \lim_{n \to \infty} \left(\frac {n + 1} n \ln n - 1 + \frac 1 n - \ln n \right) \\
\exp \lim_{n \to \infty} \left(-1 + \frac 1 n \right)  & \le \exp \lim_{n \to \infty} \left(\frac 1 n \sum _{k = 2} ^n \ln k - \ln n \right) \le \exp \lim_{n \to \infty} \left(\frac 1 n \ln n - 1 + \frac 1 n \right) \\
\exp(-1) & \le \exp \lim_{n \to \infty} \left(\frac 1 n \sum _{k = 2} ^n \ln k - \ln n \right) \le \exp(-1) \\
\frac 1 e & \le \lim_{n \to \infty} \frac { \sqrt[n]{n!} } n \le \frac 1 e \\
\frac 1 e & = \lim_{n \to \infty} \frac { \sqrt[n]{n!} } n \\
\lim_{n \to \infty} \frac { \sqrt[n]{n!} } n & = \frac 1 e
\end{aligned}$$
