---
aliases: []
tags:
  - date/2023/08/06
---

35. $$\lim_{x\to3}\frac{\sqrt{x+1}-2}{\sqrt{2x+3}-3}$$

> $$\begin{aligned}
\lim_{x\to3}\frac{\sqrt{x+1}-2}{\sqrt{2x+3}-3}&=\lim_{x\to3}\frac{\sqrt{x+1}-2}{\sqrt{2x+3}-3}\cdot\frac{\sqrt{2x+3}+3}{\sqrt{2x+3}+3}\\
&=\lim_{x\to3}\frac{\left(\sqrt{x+1}-2\right)\left(\sqrt{2x+3}+3\right)}{2x-6}\\
&=\lim_{x\to3}\frac{\left(\sqrt{x+1}-2\right)\left(\sqrt{2x+3}+3\right)}{2(x-3)}\cdot\frac{\sqrt{x+1}+2}{\sqrt{x+1}+2}\\
&=\lim_{x\to3}\frac{(x+1-4)\left(\sqrt{2x+3}+3\right)\left(\sqrt{x+1}+2\right)}{2(x-3)\left(\sqrt{x+1}+2\right)}\\
&=\lim_{x\to3}\frac{(x-3)\left(\sqrt{2x+3}+3\right)\left(\sqrt{x+1}+2\right)}{2(x-3)\left(\sqrt{x+1}+2\right)}\\
&=\lim_{x\to3}\frac{\left(\sqrt{2x+3}+3\right)\left(\sqrt{x+1}+2\right)}{2\left(\sqrt{x+1}+2\right)}\\
&=\frac{\left(\sqrt{2\cdot3+3}+3\right)\left(\sqrt{3+1}+2\right)}{2\left(\sqrt{3+1}+2\right)}\\
&=\frac{6\cdot4}{2\cdot4}\\
&=3
\end{aligned}$$
