---
aliases:
  - secondary 2 mathematics@2024-12-01 with solutions
tags:
  - date/2024/12/01
  - language/in/English
---

# secondary 2 mathematics@2024-12-01 with solutions

## exponents

1. Simplify $a \times a^2$.
2. Simplify $a^3 \times a^4$.
3. Simplify $a^a \times a^b$.
4. Simplify $a^5 \div a^2$.
5. Simplify $a^2 \div a^5$.
6. Simplify $\left(a^3\right)^9$.
7. Simplify $\left(a^9\right)^x$.
8. Simplify $\left(x^y\right)^x$.
9. Simplify $\left(\frac c d \right)^4$.
10. Simplify $\left(\frac {c^2} d \right)^4$.
11. Simplify $(xy)^a$.
12. Simplify $xy^a$.
13. Simplify $\left((xy)^a\right)^b$.
14. Simplify $\left(\frac {ac} {bd} \right)^e$.
15. Simplify $\left(cd^2 \left(\frac {a^2} {b^3} \right)^e\right)^f$.

## expand

1. Expand $(7 - 3y) (y - 3)$.
2. Expand $(-7w - 4) (2w - 5)$.
3. Expand $(3v + 7) (6v - 4)$.
4. Expand $(4 - 2m) (m + 6)$.
5. Expand $(1 - 3x) (3x + 3)$.
6. Expand $4y (7y + 5) (7y + 7)$.
7. Expand $2 (-7n - 6) (-n - 5) n$.
8. Expand $21 s^2 (3s + 7)$.
9. Expand $-6v \left(35v^2 - 39v - 14\right)$.
10. Expand $7w (3w + 2) (4w + 5) (7w + 6)$.

## factor

1. Factor $a^2 - b^2$.
2. Factor $a^2 - 2a - 15$.
3. Factor $a^2 + a - 20$.
4. Factor $n^2 - 10n + 21$.
5. Factor $2y^2 + 16y + 14$.
6. Factor $n^2 + 6n + 5$.
7. Factor $x^2 - 5xz - 6z^2$.
8. Factor $3m^2 + 12mn - 36n^2$.
9. Factor $u^4 + 8u^2 + 15$.
10. Factor $m^4 + 2m^2 n^2 + n^4$.
11. Factor $(3x)^3 - (4y)^3$.
12. Factor $(3z)^3 + (4w)^3$.
13. Factor $27a^3 - 64b^3$.
14. Factor $27c^3 + 64 d^3$.
15. Factor $a^2 + 2ab + b^2$.
16. Factor $4c^2 + 4cd + d^2$.
17. Factor $8e^2 + 8ef + 2f^2$.
18. Factor $v^3 - v^2 - 6v$.
19. Factor $2a^4 + 12a^3 + 16a^2$.
20. Factor $2n^4m - 22n^2m^2 + 56m^3$.

---

## exponents (solutions)

1. $a \times a^2 = a^{1 + 2} = a^3$
2. $a^3 \times a^4 = a^{3 + 4} = a^7$
3. $a^a \times a^b = a^{a + b}$
4. $a^5 \div a^2 = a^{5 - 2} = a^3$
5. $a^2 \div a^5 = \frac 1 {a^{5 - 2} } = \frac 1 {a^3}$
6. $\left(a^3\right)^9 = a^{3 \times 9} = a^{27}$
7. $\left(a^9\right)^x = a^{9 \times x} = a^{9x}$
8. $\left(x^y\right)^x = x^{y \times x} = x^{yx}$
9. $\left(\frac c d\right)^4 = \frac {c^4} {d^4}$
10. $\left(\frac {c^2} d\right)^4 = \frac {\left(c^2\right)^4} {d^4} = \frac {c^{2 \times 4} } {d^4} = \frac {c^8} {d^4}$
11. $(xy)^a = x^a y^a$
12. $xy^a$ is already simplified.
13. $\left((xy)^a\right)^b = (xy)^{a \times b} = (xy)^{ab} = x^{ab} y^{ab}$
14. $\left(\frac {ac} {bd}\right)^e = \frac {(ac)^e} {(bd)^e} = \frac {a^e c^e} {b^e d^e}$
15. $$\begin{aligned} & \phantom = \left(cd^2 \left(\frac {a^2} {b^3} \right)^e \right)^f \\ & = \left(cd^2 \left(\frac {\left(a^2\right)^e} {\left(b^3\right)^e} \right) \right)^f \\ & = \left(cd^2 \left(\frac {a^{2e} } {b^{3e} } \right) \right)^f \\ & = \left(\frac {c d^2 a^{2e} } {b^{3e} } \right)^f \\ & = \frac {\left(c d^2 a^{2e}\right)^f} {\left(b^{3e}\right)^f} \\ & = \frac {c^f d^{2f} e^{2ef} } {b^{3ef} } \end{aligned}$$

## expand (solutions)

1. $(7 - 3y) (y - 3) = 7y - 21 - 3y^2 + 9y = -3y^2 + 16y - 21$
2. $(-7w - 4) (2w - 5) = -14w^2 + 35w - 8w + 20 = -14w^2 + 27w + 20$
3. $(3v + 7) (6v - 4) = 18v^2 - 12v + 42v - 28 = 18v^2 + 30v - 28$
4. $(4 - 2m) (m + 6) = 4m + 24 - 2m^2 - 12m = -2m^2 -8m + 24$
5. $(1 - 3x) (3x + 3) = 3x + 3 - 9x^2 - 9x = -9x^2 - 6x + 3$
6. $$\begin{aligned} & \phantom = 4y (7y + 5) (7y + 7) \\ & = 4y \left(49y^2 + 49y + 35y + 35\right) \\ & = 4y \left(49y^2 + 84y + 35\right) \\ & = 196y^3 + 336y^2 + 140y \end{aligned}$$
7. $$\begin{aligned} & \phantom = 2 (-7n - 6) (-n - 5) n \\ & = 2n (-7n - 6) (-n - 5) \\ & = 2n \left(7n^2 + 35n + 6n + 30 \right) \\ & = 2n \left(7n^2 + 41n + 30\right) \\ & = 14n^3 + 82n^2 + 60n \end{aligned}$$
8. $21 s^2 (3s + 7) = 63s^3 + 147s^2$
9. $-6v \left(35v^2 - 39v - 14\right) = -210v^3 + 234v^2 + 84v$
10. $$\begin{aligned} & \phantom = 7w (3w + 2) (4w + 5) (7w + 6) \\ & = 7w (3w + 2) \left(28w^2 + 24w + 35w + 30\right) \\ & = 7w (3w + 2) \left(28w^2 + 59w + 30\right) \\ & = 7w \left(84w^3 + 177w^2 + 90w + 56w^2 + 118w + 60\right) \\ & = 7w \left(84w^3 + 233w^2 + 208w + 60\right) \\ & = 588w^4 + 1631w^3 + 1456w^2 + 420w \end{aligned}$$

## factor (solutions)

1. $a^2 - b^2 = (a + b) (a - b)$
2. $a^2 - 2a - 15 = (a + 3) (a - 5)$
3. $a^2 + a - 20 = (a + 5) (a - 4)$
4. $n^2 - 10n + 21 = (n - 3) (n - 7)$
5. $2y^2 + 16y + 14 = 2\left(y^2 + 8y + 7\right) = 2 (y + 7) (y + 1)$
6. $n^2 + 6n + 5 = (n + 5) (n + 1)$
7. $x^2 - 5xz - 6z^2 = (x + z) (x - 6z)$
8. $3m^2 + 12mn - 36n^2 = 3 \left(m^2 + 4mn - 12n^2 \right) = 3 (m + 6n) (m - 2n)$
9. $u^4 + 8u^2 + 15 = \left(u^2\right)^2 + 8\left(u^2\right) + 15 = \left(u^2 + 5\right) \left(u^2 + 3\right)$
10. $m^4 + 2m^2 n^2 + n^4 = \left(m^2\right)^2 + 2\left(m^2\right)\left(n^2\right) + \left(n^2\right)^2 = \left(m^2 + n^2\right)^2$
11. $$\begin{aligned} & \phantom = (3x)^3 - (4y)^3 \\ & = (3x - 4y) \left((3x)^2 + (3x) (4y) + (4y)^2 \right) \\ & = (3x - 4y) \left(9x^2 + 12xy + 16y^2 \right) \end{aligned}$$
12. $$\begin{aligned} & \phantom = (3z)^3 + (4w)^3 \\ & = (3z + 4w) \left((3z)^2 - (3z) (4w) + (4w)^2 \right) \\ & = (3z + 4w) \left(9z^2 - 12zw + 16w^2 \right)\end{aligned}$$
13. $$\begin{aligned} & \phantom = 27a^3 - 64b^3 \\ & = 3^3 a^3 - 4^3 b^3 \\ & = (3a)^3 - (4b)^3 \\ & = (3a - 4b) \left((3a)^2 + (3a) (4b) + (4b)^2 \right) \\ & = (3a - 4b) \left(9a^2 + 12ab + 16b^2 \right) \end{aligned}$$
14. $$\begin{aligned} & \phantom = 27c^3 + 64 d^3 \\ & = 3^3 c^3 + 4^3 d^3 \\ & = (3c)^3 + (4d)^3 \\ & = (3c + 4d) \left((3c)^2 - (3c) (4d) + (4d)^2 \right) \\ & = (3c + 4d) \left(9c^2 - 12cd + 16d^2 \right) \end{aligned}$$
15. $a^2 + 2ab + b^2 = (a + b)^2$
16. $4c^2 + 4cd + d^2 = (2c)^2 + 2 (2c) d + d^2 = (2c + d)^2$
17. $8e^2 + 8ef + 2f^2 = 2\left(4e^2 + 4ef + f^2 \right) = 2\left((2e)^2 + 2 (2e) f + f^2 \right) = 2 (2e + f)^2$
18. $v^3 - v^2 - 6v = v\left(v^2 - v - 6 \right) = v (v + 2) (v - 3)$
19. $2a^4 + 12a^3 + 16a^2 = 2a^2 \left(a^2 + 6a + 8 \right) = 2a^2 (a + 4) (a + 2)$
20. $$\begin{aligned} & \phantom = 2n^4m - 22n^2m^2 + 56m^3 \\ & = 2m \left(n^4 - 11 n^2 m + 28m\right) \\ & = 2m \left(\left(n^2\right)^2 - 11 \left(n^2\right) m + 28m^2 \right) \\ & = 2m \left(n^2 - 4m\right) \left(n^2 - 7m^2\right) \end{aligned}$$
