---
aliases: []
tags:
  - date/2024/10/29
  - language/in/English
---

# maybe later

$$\begin{aligned}
U(n) & := T\left(3^n\right) \\
U(\log_3 n) & := T(n) \\
\\
T(n) & = 3T(n / 3) + \frac n {\log n} \\
T\left(3^n\right) & = 3T\left(3^n / 3\right) + \frac {3^n} {\log\left(3^n\right)} \\
& = 3T\left(3^{n - 1}\right) + \frac {3^n} {n \log 3} \\
\\
U(n) & = 3U(n - 1) + \frac {3^n} {n \log 3} \\
U(n + 1) & = 3U(n) + \frac{3^{n + 1} } {(n + 1) \log 3} \\
n U(n) & = 3nU(n - 1) + \frac {3^n} {\log 3} \\
n U(n) & = 3U(n - 1) + 3(n - 1)U(n - 1) + \frac {3^n} {\log 3} \\
\\
xG'(x) & = 3xG(x) + x^2G'(x) + \frac 1 {\log 3} \frac 1 {1 - 3x} \\
(x - 1)xG'(x) + 3xG(x) & = -\frac 1 {\log 3} \frac 1 {1 - 3x} \\
(x - 1)x \frac {\mathrm{d} G(x)} {\mathrm dx} + 3x G(x) & = -\frac 1 {\log 3} \frac 1 {1 - 3x} \\
\\
(x - 1)x \frac {\mathrm{d} \tilde G(x)} {\mathrm dx} + 3x \tilde G(x) & = 0 \\
(x - 1)x \frac {\mathrm{d} \tilde G(x)} {\mathrm dx} & = -3x \tilde G(x) \\
\frac 1 {\tilde G(x)} \,\mathrm{d} \tilde G(x) & = \frac {-3x} {(x - 1) x} \,\mathrm{d}x \\
\ln \lvert \tilde G(x) \rvert & = -3 \ln \lvert x - 1 \rvert + C \\
\tilde G(x) & = C (x - 1)^{-3} \\
\\
G(x) & = -\frac {(x - 1)^{-3} } {\log 3} \int \frac {(x - 1)^3} {1 - 3x} \! \,\mathrm{d}x \\
& = \frac {(x - 1)^{-3} } {\log 3} \int \frac {(1 - x)^3} {1 - 3x} \! \,\mathrm{d}x \\
& = \frac {(x - 1)^{-3} } {\log 3} \left(-\frac {24 \ln \lvert 3x - 1 \rvert - 27x^3 + 108 x^2 - 171x} {243} + C \right) \\
& = (1 - x)^{-3} \left(\frac {24 \ln \lvert 3x - 1 \rvert - 27x^3 + 108 x^2 - 171x} {243 \log 3} + C \right) \\
U(n) & = \frac {\left[x^n\right]} {243 \log 3} \left(\sum_n \binom {2 + n} 2 x^n \right) \left(24 \sum_{n \ge 1} \frac {3^n} n x^n - 27x^3 + 108x^2 -171x + C \right) \\
& \approx -\frac {24} {243 \log 3} \sum_{k = 1}^{n - 1} \binom {2 + k} 2 \frac {3^{n - k} } {n - k} \\
& ??? \\
\\
E'(x) & = 3E(x) + \frac {e^{3x} } {x \log 3} \\
E'(x) - 3E(x) & = \frac {e^{3x} } {x \log 3} \\
\\
\tilde E'(x) - 3 \tilde E(x) & = 0 \\
u - 3 & = 0 \\
u & = 3 \\
\tilde E(x) & = C_1 e^{3x} \\
\\
E(x) & = e^{3x} \int \! \frac {\frac {e^{3x} } {x \log 3} } {e^{3x} } \,\mathrm{d}x \\
& = \frac {e^{3x} } {\log 3} \int \! \frac 1 x \,\mathrm{d}x \\
& = \frac {e^{3x} } {\log 3} (\ln x + C_1) \\
& ???
\end{aligned}$$
